Adjust Sorts

matching-logic/src/Theories/Sorts.v
@@ -16,6 +16,7 @@ Require Import MatchingLogic.Theories.Definedness.
 Import MatchingLogic.Syntax.Notations.
 Import MatchingLogic.Syntax.BoundVarSugar.
 Import MatchingLogic.Semantics.Notations.
+Import MatchingLogic.IndexManipulation.
 Import MatchingLogic.DerivedOperators.Notations.
 
 
@@ -57,27 +58,52 @@ Section sorts.
     |}.
 
   Definition patt_forall_of_sort (sort phi : Pattern) : Pattern :=
-    patt_forall ((patt_in (patt_bound_evar 0) (patt_inhabitant_set sort)) ---> phi).
+    patt_forall ((patt_in (patt_bound_evar 0) (patt_inhabitant_set (nest_ex sort))) ---> phi).
 
   Definition patt_exists_of_sort (sort phi : Pattern) : Pattern :=
-    patt_exists ((patt_in (patt_bound_evar 0) (patt_inhabitant_set sort)) and phi).
+    patt_exists ((patt_in (patt_bound_evar 0) (patt_inhabitant_set (nest_ex sort))) and phi).
 
   Lemma bevar_subst_forall_of_sort s ψ (wfcψ : well_formed_closed ψ) db ϕ :
-    bevar_subst (patt_forall_of_sort s ϕ) ψ db = patt_forall_of_sort (bevar_subst s ψ (S db)) (bevar_subst ϕ ψ (S db)).
-  Proof. reflexivity. Qed.
+    bevar_subst (patt_forall_of_sort s ϕ) ψ db = patt_forall_of_sort (bevar_subst s ψ db) (bevar_subst ϕ ψ (S db)).
+  Proof.
+    unfold patt_forall_of_sort.
+    repeat (rewrite simpl_bevar_subst';[assumption|]).
+    simpl. unfold nest_ex. replace (S db) with (db + 1) by lia. rewrite nest_ex_gt; auto. lia.
+  Qed.
 
   Lemma bsvar_subst_forall_of_sort s ψ (wfcψ : well_formed_closed ψ) db ϕ :
     bsvar_subst (patt_forall_of_sort s ϕ) ψ db = patt_forall_of_sort (bsvar_subst s ψ db) (bsvar_subst ϕ ψ db).
-  Proof. reflexivity. Qed.
+  Proof.
+    unfold patt_forall_of_sort.
+    repeat (rewrite simpl_bsvar_subst';[assumption|]).
+    simpl.
+    rewrite bsvar_subst_nest_ex_aux_comm.
+    { unfold well_formed_closed in wfcψ. destruct_and!. assumption. }
+    reflexivity.
+  Qed.
 
   Lemma bevar_subst_exists_of_sort s ψ (wfcψ : well_formed_closed ψ) db ϕ :
-    bevar_subst (patt_exists_of_sort s ϕ) ψ db = patt_exists_of_sort (bevar_subst s ψ (S db)) (bevar_subst ϕ ψ (S db)).
-  Proof. reflexivity. Qed.
+    bevar_subst (patt_exists_of_sort s ϕ) ψ db = patt_exists_of_sort (bevar_subst s ψ db) (bevar_subst ϕ ψ (db+1)).
+  Proof.
+    unfold patt_exists_of_sort.
+    repeat (rewrite simpl_bevar_subst';[assumption|]).
+    (* TODO rewrite all _+1 to 1+_ *)
+    rewrite PeanoNat.Nat.add_comm. simpl.
+    unfold nest_ex.
+    simpl. unfold nest_ex. replace (S db) with (db + 1) by lia. rewrite nest_ex_gt; auto. lia.
+  Qed.
 
   Lemma bsvar_subst_exists_of_sort s ψ (wfcψ : well_formed_closed ψ) db ϕ :
     bsvar_subst (patt_exists_of_sort s ϕ) ψ db = patt_exists_of_sort (bsvar_subst s ψ db) (bsvar_subst ϕ ψ db).
-  Proof. reflexivity. Qed.
-
+  Proof.
+    unfold patt_exists_of_sort.
+    repeat (rewrite simpl_bsvar_subst';[assumption|]).
+    simpl.
+    rewrite bsvar_subst_nest_ex_aux_comm.
+    { unfold well_formed_closed in wfcψ. destruct_and!. assumption. }
+    reflexivity.
+  Qed.
+    
   #[global]
    Instance EBinder_forall_of_sort s : EBinder (patt_forall_of_sort s) _ _:=
     {|
@@ -95,27 +121,27 @@ Section sorts.
   (* TODO patt_forall_of_sort and patt_exists_of_sorts are duals - a lemma *)
 
   (* TODO a lemma about patt_forall_of_sort *)
-
+  
   Definition patt_total_function(phi from to : Pattern) : Pattern :=
-    patt_forall_of_sort from (patt_exists_of_sort to (patt_equal (patt_app phi b1) b0)).
+    patt_forall_of_sort from (patt_exists_of_sort (nest_ex to) (patt_equal (patt_app (nest_ex (nest_ex phi)) b1) b0)).
 
   Definition patt_partial_function(phi from to : Pattern) : Pattern :=
-    patt_forall_of_sort from (patt_exists_of_sort to (patt_subseteq (patt_app phi b1) b0)).
+    patt_forall_of_sort from (patt_exists_of_sort (nest_ex to) (patt_subseteq (patt_app (nest_ex (nest_ex phi)) b1) b0)).
 
 
   (* Assuming `f` is a total function, says it is injective on given domain. Does not quite work for partial functions. *)
   Definition patt_total_function_injective f from : Pattern :=
-    patt_forall_of_sort from (patt_forall_of_sort from (patt_imp (patt_equal (patt_app f b1) (patt_app f b0)) (patt_equal b1 b0))).
+    patt_forall_of_sort from (patt_forall_of_sort (nest_ex from) (patt_imp (patt_equal (patt_app (nest_ex (nest_ex f)) b1) (patt_app (nest_ex (nest_ex f)) b0)) (patt_equal b1 b0))).
 
   (* Assuming `f` is a partial function, says it is injective on given domain. Works for total functions, too. *)
   Definition patt_partial_function_injective f from : Pattern :=
     patt_forall_of_sort
       from
       (patt_forall_of_sort
-         from
+         (nest_ex from)
          (patt_imp
-            (patt_not (patt_equal (patt_app f b1) patt_bott ))
-            (patt_imp (patt_equal (patt_app f b1) (patt_app f b0)) (patt_equal b1 b0)))).
+            (patt_not (patt_equal (patt_app (nest_ex (nest_ex f)) b1) patt_bott ))
+            (patt_imp (patt_equal (patt_app (nest_ex (nest_ex f)) b1) (patt_app (nest_ex (nest_ex f)) b0)) (patt_equal b1 b0)))).
   
 
   Section with_model.
@@ -130,14 +156,13 @@ Section sorts.
     Lemma pattern_interpretation_forall_of_sort_predicate s ϕ ρₑ ρₛ:
       let x := fresh_evar ϕ in
       M_predicate M (evar_open 0 x ϕ) ->
-      well_formed_closed_ex_aux s 0 ->
       pattern_interpretation ρₑ ρₛ (patt_forall_of_sort s ϕ) = ⊤
       <-> (∀ m : Domain M, m ∈ Minterp_inhabitant s ρₑ ρₛ ->
                            pattern_interpretation (update_evar_val x m ρₑ) ρₛ (evar_open 0 x ϕ) = ⊤).
     Proof.
-      intros x Hpred Hwfs.
+      intros x Hpred.
       unfold patt_forall_of_sort.
-      assert (Hsub: is_subformula_of_ind ϕ (patt_in b0 (patt_inhabitant_set s) ---> ϕ)).
+      assert (Hsub: is_subformula_of_ind ϕ (patt_in b0 (patt_inhabitant_set (nest_ex s)) ---> ϕ)).
       { apply sub_imp_r. apply sub_eq. reflexivity.  }
       rewrite pattern_interpretation_forall_predicate.
       2: {
@@ -151,8 +176,8 @@ Section sorts.
           eapply evar_fresh_in_subformula. apply Hsub. apply set_evar_fresh_is_fresh.
       }
       subst x.
-      remember (patt_in b0 (patt_inhabitant_set s) ---> ϕ) as Bigϕ.
-      assert (Hfresh: fresh_evar Bigϕ ∉ free_evars (patt_sym (inj inhabitant) $ s)).
+      remember (patt_in b0 (patt_inhabitant_set (nest_ex s)) ---> ϕ) as Bigϕ.
+      assert (Hfresh: fresh_evar Bigϕ ∉ free_evars (patt_sym (inj inhabitant) $ (nest_ex s))).
       { rewrite HeqBigϕ.
         unfold patt_inhabitant_set.
         fold (evar_is_fresh_in (fresh_evar (patt_in b0 (sym inhabitant $ s) ---> ϕ)) (patt_sym (inj inhabitant) $ s)).
@@ -169,7 +194,7 @@ Section sorts.
 
       remember (patt_in b0 (patt_inhabitant_set s) ---> ϕ) as Bigϕ'.
       assert (HfreeBigϕ: free_evars Bigϕ = free_evars Bigϕ').
-      { subst. reflexivity. }
+      { subst. simpl. unfold nest_ex. rewrite free_evars_nest_ex_aux. reflexivity. }
       assert (HfreshBigϕ: fresh_evar Bigϕ = fresh_evar Bigϕ').
       { unfold fresh_evar. rewrite HfreeBigϕ. reflexivity. }
       clear HfreeBigϕ.
@@ -187,68 +212,75 @@ Section sorts.
         specialize (H m).
         (*rewrite -interpretation_fresh_evar_subterm.*)
         rewrite -(@interpretation_fresh_evar_subterm _ _ _ Bigϕ).
-        assumption.
-        rewrite -> HeqBigϕ, -> HeqBigϕ' in H.
+        rewrite HeqBigϕ in H.
         rewrite evar_open_imp in H.
-        rewrite <- HeqBigϕ', <- HeqBigϕ in H.
-
-        apply pattern_interpretation_impl_MP with (ϕ₁ := evar_open 0 (fresh_evar Bigϕ) (patt_in b0 (patt_inhabitant_set s))). exact H.
+        rewrite -HeqBigϕ in H.
+        assumption.
+        rewrite {3}HeqBigϕ in H.
+        eapply pattern_interpretation_impl_MP.
+        apply H.
+        simpl. fold evar_open.
   
         unfold Minterp_inhabitant in H'.
-        pose proof (Hfeip := @free_evar_in_patt _ _ M M_satisfies_theory (fresh_evar Bigϕ) (patt_sym (inj inhabitant) $ evar_open 0 (fresh_evar Bigϕ) s) (update_evar_val (fresh_evar Bigϕ) m ρₑ) ρₛ).
+        pose proof (Hfeip := @free_evar_in_patt _ _ M M_satisfies_theory (fresh_evar Bigϕ) (patt_sym (inj inhabitant) $ evar_open 0 (fresh_evar Bigϕ) (nest_ex s)) (update_evar_val (fresh_evar Bigϕ) m ρₑ) ρₛ).
         destruct Hfeip as [Hfeip1 _]. apply Hfeip1. clear Hfeip1.
         rewrite update_evar_val_same.
         clear H. unfold sym in H'.
         unfold Ensembles.In.
         
         rewrite pattern_interpretation_app_simpl.
+        unfold evar_open. rewrite nest_ex_same.
         rewrite pattern_interpretation_sym_simpl.
 
         rewrite pattern_interpretation_app_simpl in H'.
         rewrite pattern_interpretation_sym_simpl in H'.
-
-        rewrite evar_open_not_occur; [auto|].
-        rewrite pattern_interpretation_free_evar_independent; [solve_free_evars_inclusion 5 | exact H' ].
+        rewrite pattern_interpretation_free_evar_independent.
+        {
+          solve_free_evars_inclusion 5.
+        }
+        apply H'.
 
       - intros H m.
-        pose proof (Hfeip := @free_evar_in_patt _ _ M M_satisfies_theory (fresh_evar Bigϕ) (patt_sym (inj inhabitant) $ evar_open 0 (fresh_evar Bigϕ) s) (update_evar_val (fresh_evar Bigϕ) m ρₑ) ρₛ).
+        pose proof (Hfeip := @free_evar_in_patt _ _ M M_satisfies_theory (fresh_evar Bigϕ) (patt_sym (inj inhabitant) $ evar_open 0 (fresh_evar Bigϕ) (nest_ex s)) (update_evar_val (fresh_evar Bigϕ) m ρₑ) ρₛ).
         destruct Hfeip as [_ Hfeip2].
-        unfold evar_open. simpl.
-        rewrite -> HeqBigϕ, -> HeqBigϕ'.
+        rewrite {3}HeqBigϕ.
+        unfold evar_open. simpl_bevar_subst. simpl.
         apply pattern_interpretation_predicate_impl.
         apply T_predicate_in. apply M_satisfies_theory.
-        intros H1. fold bevar_subst in *. rewrite -> HeqBigϕ, -> HeqBigϕ' in Hfeip2.
+        intros H1.
         specialize (Hfeip2 H1). clear H1.
         specialize (H m).
         rewrite -(@interpretation_fresh_evar_subterm _ _ _ Bigϕ) in H.
-        apply Hsub.
-        rewrite -> HeqBigϕ, -> HeqBigϕ' in H.
-        apply H. clear H.
-        
+        apply Hsub. apply H. clear H.
+
         unfold Minterp_inhabitant.
         unfold Ensembles.In in Hfeip2. unfold sym.
+
+
         rewrite pattern_interpretation_app_simpl in Hfeip2.
+        unfold evar_open in Hfeip2. rewrite nest_ex_same in Hfeip2.
         rewrite pattern_interpretation_sym_simpl in Hfeip2.
 
         rewrite pattern_interpretation_app_simpl.
         rewrite pattern_interpretation_sym_simpl.
         rewrite update_evar_val_same in Hfeip2.
-        rewrite evar_open_not_occur in Hfeip2; [auto|].
-        rewrite pattern_interpretation_free_evar_independent in Hfeip2; auto.
-        unfold evar_is_fresh_in, fresh_evar. cbn.
-        set_solver.
+        rewrite pattern_interpretation_free_evar_independent in Hfeip2.
+        {
+          solve_free_evars_inclusion 5.
+        }
+        apply Hfeip2.
     Qed.
 
     Lemma pattern_interpretation_exists_of_sort_predicate s ϕ ρₑ ρₛ:
       let x := fresh_evar ϕ in
-      M_predicate M (evar_open 0 x ϕ) -> well_formed_closed_ex_aux s 0 ->
+      M_predicate M (evar_open 0 x ϕ) ->
       pattern_interpretation ρₑ ρₛ (patt_exists_of_sort s ϕ) = ⊤
       <-> (∃ m : Domain M, m ∈ Minterp_inhabitant s ρₑ ρₛ /\
                            pattern_interpretation (update_evar_val x m ρₑ) ρₛ (evar_open 0 x ϕ) = ⊤).
     Proof.
-      intros x Hpred WFs.
+      intros x Hpred.
       unfold patt_exists_of_sort.
-      assert (Hsub: is_subformula_of_ind ϕ (patt_in b0 (patt_inhabitant_set s) and ϕ)).
+      assert (Hsub: is_subformula_of_ind ϕ (patt_in b0 (patt_inhabitant_set (nest_ex s)) and ϕ)).
       { unfold patt_and. unfold patt_or.  apply sub_imp_l. apply sub_imp_r. apply sub_imp_l. apply sub_eq. reflexivity. }
       rewrite -> pattern_interpretation_exists_predicate_full.
       2: {
@@ -262,8 +294,8 @@ Section sorts.
           eapply evar_fresh_in_subformula. apply Hsub. apply set_evar_fresh_is_fresh.
       }
       subst x.
-      remember (patt_in b0 (patt_inhabitant_set s) and ϕ) as Bigϕ.
-      assert (Hfresh: fresh_evar Bigϕ ∉ free_evars (patt_sym (inj inhabitant) $ s)).
+      remember (patt_in b0 (patt_inhabitant_set (nest_ex s)) and ϕ) as Bigϕ.
+      assert (Hfresh: fresh_evar Bigϕ ∉ free_evars (patt_sym (inj inhabitant) $ (nest_ex s))).
       { rewrite HeqBigϕ.
         unfold patt_inhabitant_set.
         fold (evar_is_fresh_in (fresh_evar (patt_in b0 (sym inhabitant $ s) and ϕ)) (patt_sym (inj inhabitant) $ s)).
@@ -282,7 +314,7 @@ Section sorts.
 
       remember (patt_in b0 (patt_inhabitant_set s) and ϕ) as Bigϕ'.
       assert (HfreeBigϕ: free_evars Bigϕ = free_evars Bigϕ').
-      { subst. reflexivity. }
+      { subst. simpl. unfold nest_ex. rewrite free_evars_nest_ex_aux. reflexivity. }
       assert (HfreshBigϕ: fresh_evar Bigϕ = fresh_evar Bigϕ').
       { unfold fresh_evar. rewrite HfreeBigϕ. reflexivity. }
       clear HfreeBigϕ.
@@ -300,40 +332,41 @@ Section sorts.
         exists m.
         rewrite -(@interpretation_fresh_evar_subterm _ _ _ Bigϕ).
         assumption.
-        simpl in H. rewrite -> HeqBigϕ, -> HeqBigϕ' in H.
+        rewrite {3}HeqBigϕ in H.
 
         apply pattern_interpretation_and_full in H.
-        fold bevar_subst in H.
+        fold evar_open in H.
         destruct H as [H1 H2].
-        split. 2:rewrite -> HeqBigϕ, -> HeqBigϕ'; apply H2. clear H2.
+        split. 2: apply H2. clear H2.
         unfold Minterp_inhabitant.
-        pose proof (Hfeip := @free_evar_in_patt _ _ M M_satisfies_theory (fresh_evar Bigϕ) (patt_sym (inj inhabitant) $ evar_open 0 (fresh_evar Bigϕ) s) (update_evar_val (fresh_evar Bigϕ) m ρₑ) ρₛ).
+        pose proof (Hfeip := @free_evar_in_patt _ _ M M_satisfies_theory (fresh_evar Bigϕ) (patt_sym (inj inhabitant) $ evar_open 0 (fresh_evar Bigϕ) (nest_ex s)) (update_evar_val (fresh_evar Bigϕ) m ρₑ) ρₛ).
         destruct Hfeip as [_ Hfeip2].
 
-        rewrite -> HeqBigϕ, -> HeqBigϕ' in Hfeip2.
         apply Hfeip2 in H1. clear Hfeip2.
         rewrite update_evar_val_same in H1.
         unfold sym.
         unfold Ensembles.In in H1.
 
         rewrite pattern_interpretation_app_simpl in H1.
+        unfold evar_open in H1.
+        rewrite nest_ex_same in H1.
         rewrite pattern_interpretation_sym_simpl in H1.
 
         rewrite pattern_interpretation_app_simpl.
         rewrite pattern_interpretation_sym_simpl.
-        rewrite evar_open_not_occur in H1; [auto|].
-        rewrite pattern_interpretation_free_evar_independent in H1; auto.
-        unfold evar_is_fresh_in, fresh_evar. cbn.
-        set_solver.
-        
+        rewrite pattern_interpretation_free_evar_independent in H1.
+        {
+          solve_free_evars_inclusion 5.
+        }
+        apply H1.
+
       - intros [m [H1 H2] ]. exists m.
-        pose proof (Hfeip := @free_evar_in_patt _ _ M M_satisfies_theory (fresh_evar Bigϕ) (patt_sym (inj inhabitant) $ evar_open 0 (fresh_evar Bigϕ) s) (update_evar_val (fresh_evar Bigϕ) m ρₑ) ρₛ).
+        pose proof (Hfeip := @free_evar_in_patt _ _ M M_satisfies_theory (fresh_evar Bigϕ) (patt_sym (inj inhabitant) $ evar_open 0 (fresh_evar Bigϕ) (nest_ex s)) (update_evar_val (fresh_evar Bigϕ) m ρₑ) ρₛ).
         destruct Hfeip as [Hfeip1 _].
-        rewrite -> HeqBigϕ, -> HeqBigϕ'.
-        apply pattern_interpretation_and_full. fold bevar_subst.
+        rewrite {3}HeqBigϕ.
+        apply pattern_interpretation_and_full. fold evar_open.
         split.
-        + rewrite -> HeqBigϕ, -> HeqBigϕ' in Hfeip1.
-          apply Hfeip1. clear Hfeip1.
+        + apply Hfeip1. clear Hfeip1.
           unfold Ensembles.In.
           rewrite -> update_evar_val_same.
           unfold Minterp_inhabitant in H1. unfold sym in H1.
@@ -342,12 +375,16 @@ Section sorts.
           rewrite pattern_interpretation_sym_simpl in H1.
 
           rewrite pattern_interpretation_app_simpl.
+          unfold evar_open. rewrite nest_ex_same.
           rewrite pattern_interpretation_sym_simpl.
-          rewrite evar_open_not_occur; [auto|].
-          rewrite pattern_interpretation_free_evar_independent; [set_solver | exact H1 ].
+          rewrite pattern_interpretation_free_evar_independent.
+          {
+            solve_free_evars_inclusion 5.
+          }
+          apply H1.
         + rewrite -(@interpretation_fresh_evar_subterm _ _ _ Bigϕ) in H2.
           apply Hsub.
-          rewrite -> HeqBigϕ, -> HeqBigϕ' in H2. apply H2.
+          apply H2.
     Qed.
 
 
@@ -394,25 +431,26 @@ Section sorts.
     Qed.
 
     Hint Resolve M_predicate_forall_of_sort : core.
-    
+
     Lemma interp_total_function f s₁ s₂ ρₑ ρₛ :
-      well_formed_closed_ex_aux s₁ 0 -> well_formed_closed_ex_aux s₂ 0 ->
-      well_formed_closed_ex_aux f 0 ->
       @pattern_interpretation Σ M ρₑ ρₛ (patt_total_function f s₁ s₂) = ⊤ <->
       @is_total_function Σ M f (Minterp_inhabitant s₁ ρₑ ρₛ) (Minterp_inhabitant s₂ ρₑ ρₛ) ρₑ ρₛ.
     Proof.
-      intros WF1 WF2 WFF.
       unfold is_total_function.
-      rewrite pattern_interpretation_forall_of_sort_predicate; auto.
+      rewrite pattern_interpretation_forall_of_sort_predicate.
       2: { eauto. }
 
       unfold evar_open. simpl_bevar_subst.
-      remember (fresh_evar (patt_exists_of_sort s₂ (patt_equal (f $ b1) b0))) as x'.
+      remember (fresh_evar (patt_exists_of_sort (nest_ex s₂) (patt_equal ((nest_ex (nest_ex f)) $ b1) b0))) as x'.
+      rewrite [nest_ex s₂]/nest_ex.
+      unfold nest_ex. repeat rewrite nest_ex_same.
+      rewrite fuse_nest_ex_same. rewrite nest_ex_same_general. 1-2: lia. simpl.
+      rewrite -/(nest_ex s₂).
 
       apply all_iff_morphism.
       unfold pointwise_relation. intros m₁.
       apply all_iff_morphism. unfold pointwise_relation. intros Hinh1.
-      
+
       rewrite pattern_interpretation_exists_of_sort_predicate.
       2: {
         unfold evar_open. simpl_bevar_subst.
@@ -424,36 +462,30 @@ Section sorts.
       rewrite 2!pattern_interpretation_app_simpl.
       rewrite 2!pattern_interpretation_sym_simpl.
       rewrite pattern_interpretation_free_evar_independent.
-      { rewrite Heqx'. rewrite bevar_subst_not_occur; [eapply well_formed_closed_ex_aux_ind;
-                               try eassumption; lia|].
-        eapply evar_is_fresh_in_richer.
-        2: apply set_evar_fresh_is_fresh.
-        cbn. rewrite !(left_id_L ∅ union). rewrite !(right_id_L ∅ union).
-        rewrite (idemp_L union). apply union_subseteq_l. } 
+      (* two subgoals *)
+      fold (evar_is_fresh_in x' (nest_ex s₂)).
 
-      assert (Hfreq: x' = fresh_evar (patt_imp s₂ f)).
+      assert (Hfreq: x' = fresh_evar (patt_imp s₂ (nest_ex (nest_ex f)))).
       { rewrite Heqx'. unfold fresh_evar. apply f_equal. simpl.
+        rewrite 2!free_evars_nest_ex_aux.
         rewrite !(left_id_L ∅ union). rewrite !(right_id_L ∅ union).
         rewrite (idemp_L union). reflexivity.
       }
-      2: { rewrite bevar_subst_not_occur; [eapply well_formed_closed_ex_aux_ind;
-                               try eassumption; lia|auto]. }
+      {
+        rewrite Hfreq.
+        unfold evar_is_fresh_in.
+        eapply evar_is_fresh_in_richer'.
+        2: apply set_evar_fresh_is_fresh'. solve_free_evars_inclusion 5.
+      }
 
-      rewrite Hfreq.
-      (* unfold evar_is_fresh_in.
-      rewrite free_evars_nest_ex_aux.
-      fold (evar_is_fresh_in (fresh_evar (s₂ ---> f)) s₂).
-      eapply evar_fresh_in_subformula'. 2: apply set_evar_fresh_is_fresh.
-      simpl. rewrite is_subformula_of_refl. rewrite orb_true_r. auto. *)
-      (* one subgoal remains *)
+      apply and_iff_morphism; auto.
 
-      apply and_iff_morphism.
-      rewrite bevar_subst_not_occur; [eapply well_formed_closed_ex_aux_ind;
-                               try eassumption; lia|auto].
+      unfold nest_ex.
+      unfold evar_open. simpl_bevar_subst.
+      repeat rewrite nest_ex_same.
 
-      unfold evar_open. simpl.
 
-      remember (fresh_evar (patt_equal (f $ patt_free_evar x') b0)) as x''.
+      remember (fresh_evar (patt_equal (nest_ex_aux 0 1 f $ patt_free_evar x') b0)) as x''.
 
       rewrite equal_iff_interpr_same. 2: apply M_satisfies_theory.
       simpl. rewrite pattern_interpretation_free_evar_simpl.
@@ -464,59 +496,29 @@ Section sorts.
       (*  Hx''neqx' : x'' ≠ x'
           Hx''freeinf : x'' ∉ free_evars f
        *)
-      pose proof (HB := @set_evar_fresh_is_fresh' _ (free_evars(patt_equal (f $ patt_free_evar x') b0))).
-      pose proof (Heqx''2 := Heqx'').
-      unfold fresh_evar in Heqx''2.
-      rewrite -Heqx''2 in HB.
-      simpl in HB.
-      rewrite !(left_id_L ∅ union) in HB.
-      rewrite !(right_id_L ∅ union) in HB.
-      apply sets.not_elem_of_union in HB. destruct HB as [HB _].
-      apply sets.not_elem_of_union in HB. destruct HB as [Hx''freeinf Hx''neqx'].
-      apply not_elem_of_singleton_1 in Hx''neqx'.
-
-      (* Hx'fr : x' ∉ free_evars f *)
-      pose proof (Hx'fr := @set_evar_fresh_is_fresh _ (patt_exists_of_sort s₂ (patt_equal (f $ b1) b0))).
-      rewrite -Heqx' in Hx'fr.
-      unfold evar_is_fresh_in in Hx'fr. simpl in Hx'fr.
-      rewrite !(left_id_L ∅ union) in Hx'fr.
-      rewrite !(right_id_L ∅ union) in Hx'fr.
-      apply sets.not_elem_of_union in Hx'fr. destruct Hx'fr as [_ Hx'fr].
-      apply sets.not_elem_of_union in Hx'fr. destruct Hx'fr as [Hx'fr _].
-
       rewrite {2}update_evar_val_comm.
-      { rewrite bevar_subst_not_occur; [eapply well_formed_closed_ex_aux_ind;
-                try eassumption; lia|auto].
-        rewrite <- Hfreq, <- Heqx''. assumption. }
-      (* do 2 rewrite -> evar_open_bound_evar. *)
-      (* repeat case_match; try lia. *)
-      (* rewrite <- Heqx''. *)
-      (*apply Hx''neqx'.*)
+      {
+        solve_fresh_neq.
+      }
       rewrite update_evar_val_same.
-      simpl.
-
       rewrite pattern_interpretation_free_evar_independent.
-      { rewrite bevar_subst_not_occur; [eapply well_formed_closed_ex_aux_ind;
-                try eassumption; lia|auto]. 
-        rewrite bevar_subst_not_occur; [eapply well_formed_closed_ex_aux_ind;
-                try eassumption; lia|auto]. 
-        rewrite <- Hfreq, <- Heqx''. assumption. }
-      (*
-      do 2 rewrite evar_open_bound_evar.
-      repeat case_match; try lia.
-      unfold nest_ex in Heqx''.
-      rewrite <- Heqx''. assumption.*)
+      {
+         rewrite Heqx''. unfold evar_is_fresh_in.
+         eapply evar_is_fresh_in_richer'.
+         2: apply set_evar_fresh_is_fresh'. cbn.
+         solve_free_evars_inclusion 5.
+      }
       rewrite pattern_interpretation_free_evar_independent.
-      all: rewrite bevar_subst_not_occur; auto. 
-      all: rewrite bevar_subst_not_occur; [eapply well_formed_closed_ex_aux_ind;
-              try eassumption; lia|auto].
-      eapply evar_is_fresh_in_richer. 2: apply set_evar_fresh_is_fresh.
-      cbn. apply union_subseteq_r.
+      {
+         rewrite Heqx'. unfold evar_is_fresh_in.
+         eapply evar_is_fresh_in_richer'.
+         2: apply set_evar_fresh_is_fresh'. cbn.
+         solve_free_evars_inclusion 5.
+      }
+      auto.
     Qed.
 
     Lemma interp_partial_function f s₁ s₂ ρₑ ρₛ :
-      well_formed_closed_ex_aux s₁ 0 -> well_formed_closed_ex_aux s₂ 0 ->
-      well_formed_closed_ex_aux f 0 ->
       @pattern_interpretation Σ M ρₑ ρₛ (patt_partial_function f s₁ s₂) = ⊤ <->
       ∀ (m₁ : Domain M),
         m₁ ∈ Minterp_inhabitant s₁ ρₑ ρₛ ->
@@ -525,26 +527,26 @@ Section sorts.
           (app_ext (@pattern_interpretation Σ M ρₑ ρₛ f) {[m₁]})
             ⊆ {[m₂]}.
     Proof.
-      intros WF1 WF2 WFF.
-      rewrite pattern_interpretation_forall_of_sort_predicate; auto.
+      rewrite pattern_interpretation_forall_of_sort_predicate.
       2: { eauto. }
 
-      unfold evar_open. simpl_bevar_subst.                                                       
-      remember (fresh_evar (patt_exists_of_sort s₂ (patt_subseteq ( f $ b1) b0))) as x'.
+      unfold evar_open. simpl_bevar_subst.
+      remember (fresh_evar (patt_exists_of_sort (nest_ex s₂) (patt_subseteq ((nest_ex (nest_ex f)) $ b1) b0))) as x'.
+      rewrite [nest_ex s₂]/nest_ex.
+      rewrite nest_ex_same.
+      unfold nest_ex.
+      rewrite fuse_nest_ex_same. rewrite nest_ex_same_general. 1-2: lia. simpl.
 
       apply all_iff_morphism.
       unfold pointwise_relation. intros m₁.
       apply all_iff_morphism. unfold pointwise_relation. intros Hinh1.
-      
-      rewrite pattern_interpretation_exists_of_sort_predicate; auto.
+
+      rewrite pattern_interpretation_exists_of_sort_predicate.
       2: {
         unfold evar_open. simpl_bevar_subst.
         apply T_predicate_subseteq; apply M_satisfies_theory.
       }
-      2: {
-        rewrite bevar_subst_not_occur; [eapply well_formed_closed_ex_aux_ind;
-                [ | exact WF2 ] |auto]; lia. 
-      }
+
       apply ex_iff_morphism. unfold pointwise_relation. intros m₂.
 
       unfold Minterp_inhabitant.
@@ -552,19 +554,31 @@ Section sorts.
       rewrite 2!pattern_interpretation_sym_simpl.
       rewrite pattern_interpretation_free_evar_independent.
       {
-         rewrite bevar_subst_not_occur; [eapply well_formed_closed_ex_aux_ind;
-                try eassumption; lia|auto].
-         rewrite Heqx'. eapply evar_is_fresh_in_richer. 2: apply set_evar_fresh_is_fresh.
-         cbn. rewrite !(left_id_L ∅ union). rewrite !(right_id_L ∅ union). apply union_subseteq_l.
-      }
-      apply and_iff_morphism.
-      rewrite bevar_subst_not_occur; [eapply well_formed_closed_ex_aux_ind;
-                [ | exact WF2 ] |auto]; lia.
-      
-      
-      remember (fresh_evar (patt_subseteq (f $ patt_free_evar x') b0)) as x''.
+        fold (evar_is_fresh_in x' (nest_ex s₂)).
 
-      rewrite subseteq_iff_interpr_subseteq. fold bevar_subst. 2: apply M_satisfies_theory.
+        assert (Hfreq: x' = fresh_evar (patt_imp s₂ (nest_ex (nest_ex f)))).
+        { rewrite Heqx'. unfold fresh_evar. apply f_equal. simpl.
+          rewrite 2!free_evars_nest_ex_aux.
+          rewrite !(left_id_L ∅ union). rewrite !(right_id_L ∅ union).
+          reflexivity.
+        }
+
+        rewrite Hfreq.
+        unfold nest_ex.
+        unfold evar_is_fresh_in.
+        eapply evar_is_fresh_in_richer'.
+         2: apply set_evar_fresh_is_fresh'. cbn.
+         solve_free_evars_inclusion 5.
+      }
+
+      apply and_iff_morphism; auto.
+
+      unfold evar_open. simpl_bevar_subst.
+      rewrite nest_ex_same.
+      simpl.
+      remember (fresh_evar (patt_subseteq (nest_ex_aux 0 1 f $ patt_free_evar x') b0)) as x''.
+
+      rewrite subseteq_iff_interpr_subseteq. 2: apply M_satisfies_theory.
       simpl. rewrite pattern_interpretation_free_evar_simpl.
       rewrite update_evar_val_same.
       rewrite pattern_interpretation_app_simpl.
@@ -573,80 +587,56 @@ Section sorts.
       (*  Hx''neqx' : x'' ≠ x'
           Hx''freeinf : x'' ∉ free_evars f
        *)
-      pose proof (HB := @set_evar_fresh_is_fresh' _ (free_evars(patt_subseteq (f $ patt_free_evar x') b0))).
-      pose proof (Heqx''2 := Heqx'').
-      unfold fresh_evar in Heqx''2.
-      rewrite -Heqx''2 in HB.
-      simpl in HB.
-      rewrite !(left_id_L ∅ union) in HB.
-      rewrite !(right_id_L ∅ union) in HB.
-      apply sets.not_elem_of_union in HB. destruct HB as [Hx''freeinf Hx''neqx'].
-      apply not_elem_of_singleton_1 in Hx''neqx'.
 
-      (* Hx'fr : x' ∉ free_evars f *)
-      pose proof (Hx'fr := @set_evar_fresh_is_fresh _ (patt_exists_of_sort s₂ (patt_subseteq (f $ b1) b0))).
-      rewrite -Heqx' in Hx'fr.
-      unfold evar_is_fresh_in in Hx'fr. simpl in Hx'fr.
-      rewrite !(left_id_L ∅ union) in Hx'fr.
-      rewrite !(right_id_L ∅ union) in Hx'fr.
-      apply sets.not_elem_of_union in Hx'fr. destruct Hx'fr as [_ Hx'fr].
-      
       rewrite {2}update_evar_val_comm.
-      { rewrite bevar_subst_not_occur; [eapply well_formed_closed_ex_aux_ind;
-                [ | exact WFF ] |auto]. lia. rewrite <- Heqx''. assumption. }
-      (*do 2 rewrite evar_open_bound_evar. cbn.
-      repeat case_match; try lia.
-      rewrite <- Heqx''. apply Hx''neqx'. *)
+      {
+        solve_fresh_neq.
+      }
       rewrite update_evar_val_same.
+      unfold nest_ex.
 
       rewrite pattern_interpretation_free_evar_independent.
-      { rewrite bevar_subst_not_occur; [eapply well_formed_closed_ex_aux_ind;
-                [ | exact WFF ] |auto]. lia.
-        rewrite bevar_subst_not_occur; [eapply well_formed_closed_ex_aux_ind;
-                [ | exact WFF ] |auto]. lia.
-        eapply evar_is_fresh_in_richer. 2: apply set_evar_fresh_is_fresh.
-         cbn. rewrite !(left_id_L ∅ union). rewrite !(right_id_L ∅ union). apply union_subseteq_l.
+      {
+         rewrite Heqx''. unfold evar_is_fresh_in.
+         eapply evar_is_fresh_in_richer'.
+         2: apply set_evar_fresh_is_fresh'. cbn.
+         solve_free_evars_inclusion 5.
       }
-      (*do 2 rewrite evar_open_bound_evar. cbn. unfold nest_ex in Heqx''.
-      repeat case_match; try lia.
-      rewrite <- Heqx''. assumption.*)
       rewrite pattern_interpretation_free_evar_independent.
-      all: rewrite bevar_subst_not_occur; [eapply well_formed_closed_ex_aux_ind;
-               try eassumption |auto].
-      2,5: rewrite bevar_subst_not_occur; [eapply well_formed_closed_ex_aux_ind;
-               try eassumption |auto].
-      3, 5: exact WFF. all: try lia.
-      all: rewrite bevar_subst_not_occur; [eapply well_formed_closed_ex_aux_ind;
-               try eassumption |auto]; lia.
+      {
+         rewrite Heqx'. unfold evar_is_fresh_in.
+         eapply evar_is_fresh_in_richer'.
+         2: apply set_evar_fresh_is_fresh'. cbn.
+         solve_free_evars_inclusion 5.
+      }
+      auto.
     Qed.
 
-    Lemma Minterp_inhabitant_evar_open_update_evar_val ρₑ ρₛ x e s m n:
-      evar_is_fresh_in x s -> well_formed_closed_ex_aux s n ->
-      m ∈ Minterp_inhabitant (evar_open n x s) (update_evar_val x e ρₑ) ρₛ
+    Lemma Minterp_inhabitant_evar_open_update_evar_val ρₑ ρₛ x e s m:
+      evar_is_fresh_in x s ->
+      m ∈ Minterp_inhabitant (evar_open 0 x (nest_ex s)) (update_evar_val x e ρₑ) ρₛ
       <-> m ∈ Minterp_inhabitant s ρₑ ρₛ.
     Proof.
-      intros Hfr Hwf.
+      intros Hfr.
       unfold Minterp_inhabitant.
       rewrite 2!pattern_interpretation_app_simpl.
       rewrite 2!pattern_interpretation_sym_simpl.
-      unfold evar_open. rewrite bevar_subst_not_occur; [ auto | ].
-      rewrite pattern_interpretation_free_evar_independent; [solve_free_evars_inclusion 5 | ]; auto.
+      unfold nest_ex, evar_open. rewrite nest_ex_same.
+      rewrite pattern_interpretation_free_evar_independent; auto.
    Qed.
 
     Lemma interp_partial_function_injective f s ρₑ ρₛ :
-      well_formed_closed_ex_aux s 0 -> well_formed_closed_ex_aux f 0 ->
       @pattern_interpretation Σ M ρₑ ρₛ (patt_partial_function_injective f s) = ⊤ <->
       ∀ (m₁ : Domain M),
         m₁ ∈ Minterp_inhabitant s ρₑ ρₛ ->
-        ∀ (m₂ : Domain M),          
+        ∀ (m₂ : Domain M),
           m₂ ∈ Minterp_inhabitant s ρₑ ρₛ ->
           (rel_of ρₑ ρₛ f) m₁ ≠ ∅ ->
           (rel_of ρₑ ρₛ f) m₁ = (rel_of ρₑ ρₛ f) m₂ ->
           m₁ = m₂.
     Proof.
-      intros WfS WfF.
       unfold patt_partial_function_injective.
-      rewrite pattern_interpretation_forall_of_sort_predicate; auto.
+      rewrite pattern_interpretation_forall_of_sort_predicate.
       2: {
         match goal with
         | [ |- M_predicate _ (evar_open _ ?x _) ] => remember x
@@ -661,48 +651,71 @@ Section sorts.
       }
       remember
       (fresh_evar
-               (patt_forall_of_sort  s
-                  (! patt_equal ( f $ b1) Bot --->
-                     patt_equal ( f $ b1) ( f $ b0) ---> patt_equal b1 b0)))
+             (patt_forall_of_sort (nest_ex s)
+                (! patt_equal (nest_ex (nest_ex f) $ b1) ⊥ --->
+                 patt_equal (nest_ex (nest_ex f) $ b1) (nest_ex (nest_ex f) $ b0) --->
+                 patt_equal b1 b0)))
       as x₁.
       apply all_iff_morphism. intros m₁.
       apply all_iff_morphism. intros Hm₁s.
 
       unfold evar_open. simpl_bevar_subst.
       rewrite pattern_interpretation_forall_of_sort_predicate. 2: { eauto 8. }
-      2: { rewrite bevar_subst_not_occur; auto.
-           eapply well_formed_closed_ex_aux_ind. 2: exact WfS. lia.
-      }
       remember
       (fresh_evar
-               (evar_open 1 x₁
-                  (! patt_equal (f $ b1) Bot --->
-                     patt_equal (f $ b1) (f $ b0) ---> patt_equal b1 b0)))
+             (! patt_equal
+                  ((nest_ex (nest_ex f)).[evar:1↦patt_free_evar x₁] $ b1.[evar:1↦patt_free_evar x₁])
+                  ⊥ --->
+              patt_equal
+                ((nest_ex (nest_ex f)).[evar:1↦patt_free_evar x₁] $ b1.[evar:1↦patt_free_evar x₁])
+                ((nest_ex (nest_ex f)).[evar:1↦patt_free_evar x₁] $ b0.[evar:1↦patt_free_evar x₁]) --->
+              patt_equal b1.[evar:1↦patt_free_evar x₁] b0.[evar:1↦patt_free_evar x₁]))
       as x₂.
-        
-      apply all_iff_morphism. intros m₂. simpl.
+
+      apply all_iff_morphism. intros m₂.
       rewrite Minterp_inhabitant_evar_open_update_evar_val.
-      repeat rewrite bevar_subst_not_occur; auto.
-      1,4: eapply well_formed_closed_ex_aux_ind; try eassumption; lia.
-      2: { rewrite Heqx₁. eapply evar_is_fresh_in_richer. 2: apply set_evar_fresh_is_fresh.
-           cbn. rewrite !(left_id_L ∅ union). rewrite !(right_id_L ∅ union). apply union_subseteq_l. }
+      2: {
+        eapply evar_is_fresh_in_richer.
+        2: { subst x₁.
+             apply set_evar_fresh_is_fresh.
+        }
+        solve_free_evars_inclusion 5.
+      }
       apply all_iff_morphism. intros Hm₂s.
       unfold evar_open. simpl_bevar_subst.
+      unfold nest_ex in *.
+      rewrite fuse_nest_ex_same in Heqx₂, Heqx₁. rewrite nest_ex_same_general in Heqx₁, Heqx₂.
+      1-2: lia.
+      rewrite fuse_nest_ex_same. rewrite nest_ex_same_general. 1-2: lia. simpl.
+      rewrite nest_ex_same.
+      simpl in Heqx₁, Heqx₂.
 
       rewrite pattern_interpretation_predicate_impl. 2: { eauto. }
       simpl.
-      rewrite pattern_interpretation_predicate_not. 2: { rewrite bevar_subst_not_occur; auto. eauto. }
+      rewrite pattern_interpretation_predicate_not. 2: { eauto. }
       rewrite equal_iff_interpr_same.
       rewrite pattern_interpretation_bott_simpl. 2: apply M_satisfies_theory.
-
-      repeat rewrite bevar_subst_not_occur; auto. simpl.
       rewrite pattern_interpretation_app_simpl.
       rewrite pattern_interpretation_free_evar_simpl.
       rewrite update_evar_val_neq.
       { solve_fresh_neq. }
       rewrite update_evar_val_same.
+      rewrite pattern_interpretation_free_evar_independent.
+      {
+         rewrite Heqx₂. unfold evar_is_fresh_in.
+         eapply evar_is_fresh_in_richer'.
+         2: apply set_evar_fresh_is_fresh'. cbn.
+         solve_free_evars_inclusion 5.
+      }
+      rewrite pattern_interpretation_free_evar_independent.
+      {
+         rewrite Heqx₁. unfold evar_is_fresh_in.
+         eapply evar_is_fresh_in_richer'.
+         2: apply set_evar_fresh_is_fresh'. cbn.
+         solve_free_evars_inclusion 5.
+      }
       fold (rel_of ρₑ ρₛ f m₁).
-      (* apply all_iff_morphism. unfold pointwise_relation. intros Hnonempty. *)
+      apply all_iff_morphism. unfold pointwise_relation. intros Hnonempty.
 
       rewrite pattern_interpretation_predicate_impl. 2: { eauto. }
       (*rewrite simpl_evar_open.*)
@@ -715,21 +728,29 @@ Section sorts.
       { solve_fresh_neq. }
       rewrite update_evar_val_same.
       unfold rel_of.
-      repeat rewrite pattern_interpretation_free_evar_independent.
-      3: apply all_iff_morphism; intros Hfm1eqfm2; clear; set_solver.
-      { eapply evar_is_fresh_in_richer. 2: apply set_evar_fresh_is_fresh.
-        cbn. rewrite !(left_id_L ∅ union). rewrite !(right_id_L ∅ union).
-        clear. set_solver.
+      rewrite pattern_interpretation_free_evar_independent.
+      {
+         rewrite Heqx₂. unfold evar_is_fresh_in.
+         eapply evar_is_fresh_in_richer'.
+         2: apply set_evar_fresh_is_fresh'. cbn.
+         solve_free_evars_inclusion 5.
       }
-      { rewrite Heqx₁. clear. eapply evar_is_fresh_in_richer. 2: apply set_evar_fresh_is_fresh. set_solver. }
+      rewrite pattern_interpretation_free_evar_independent.
+      {
+         rewrite Heqx₁. unfold evar_is_fresh_in.
+         eapply evar_is_fresh_in_richer'.
+         2: apply set_evar_fresh_is_fresh'. cbn.
+         solve_free_evars_inclusion 5.
+      }
+      apply all_iff_morphism. intros Hfm1eqfm2.
+      clear.
+      set_solver.
     Qed.
 
     Lemma interp_total_function_injective f s ρₑ ρₛ :
-      well_formed_closed_ex_aux s 0 -> well_formed_closed_ex_aux f 0 ->
       @pattern_interpretation Σ M ρₑ ρₛ (patt_total_function_injective f s) = ⊤ <->
       total_function_is_injective f (Minterp_inhabitant s ρₑ ρₛ) ρₑ ρₛ.
     Proof.
-      intros WfS WfF.
       unfold total_function_is_injective.
       unfold patt_partial_function_injective.
       rewrite pattern_interpretation_forall_of_sort_predicate.
@@ -747,8 +768,8 @@ Section sorts.
       }
       remember
       (fresh_evar
-               (patt_forall_of_sort s
-                  (patt_equal (f $ b1) (f $ b0) ---> patt_equal b1 b0)))
+               (patt_forall_of_sort (nest_ex s)
+                  (patt_equal (nest_ex (nest_ex f) $ b1) (nest_ex (nest_ex f) $ b0) ---> patt_equal b1 b0)))
       as x₁.
       apply all_iff_morphism. intros m₁.
       apply all_iff_morphism. intros Hm₁s.
@@ -764,19 +785,25 @@ Section sorts.
       }
       remember
       (fresh_evar
-               (evar_open 1 x₁
-                  (patt_equal (f $ b1) (f $ b0) ---> patt_equal b1 b0)))
+             (patt_equal
+                ((nest_ex (nest_ex f)).[evar:1↦patt_free_evar x₁] $ b1.[evar:1↦patt_free_evar x₁])
+                ((nest_ex (nest_ex f)).[evar:1↦patt_free_evar x₁] $ b0.[evar:1↦patt_free_evar x₁]) --->
+              patt_equal b1.[evar:1↦patt_free_evar x₁] b0.[evar:1↦patt_free_evar x₁]))
       as x₂.
 
       apply all_iff_morphism. intros m₂.
       rewrite Minterp_inhabitant_evar_open_update_evar_val.
-      2: {        
+      2: {
         eapply evar_is_fresh_in_richer.
         2: { subst. apply set_evar_fresh_is_fresh. }
         solve_free_evars_inclusion 5.
       }
       apply all_iff_morphism. intros Hm₂s.
-      unfold evar_open. simpl_bevar_subst.
+      unfold nest_ex, evar_open in *.
+      rewrite fuse_nest_ex_same in Heqx₂, Heqx₁. rewrite nest_ex_same_general in Heqx₁, Heqx₂.
+      1-2: lia.
+      rewrite fuse_nest_ex_same. rewrite nest_ex_same_general. 1-2: lia. simpl pred.
+      simpl_bevar_subst.
 
       rewrite pattern_interpretation_predicate_impl. 2: { eauto. }
       simpl.
@@ -791,11 +818,23 @@ Section sorts.
 
       rewrite pattern_interpretation_free_evar_simpl.
       rewrite update_evar_val_same.
+      rewrite nest_ex_same.
+      rewrite pattern_interpretation_free_evar_independent.
+      {
+         rewrite Heqx₂. unfold evar_is_fresh_in.
+         eapply evar_is_fresh_in_richer'.
+         2: apply set_evar_fresh_is_fresh'. cbn.
+         solve_free_evars_inclusion 5.
+      }
+      rewrite pattern_interpretation_free_evar_independent.
+      {
+         rewrite Heqx₁. unfold evar_is_fresh_in.
+         eapply evar_is_fresh_in_richer'.
+         2: apply set_evar_fresh_is_fresh'. cbn.
+         solve_free_evars_inclusion 5.
+      }
       fold (rel_of ρₑ ρₛ f m₁). fold (rel_of ρₑ ρₛ f m₂).
-
-      repeat rewrite bevar_subst_not_occur; auto; simpl.
-      { eapply well_formed_closed_ex_aux_ind. 2: eassumption. lia. }
-      
+      apply all_iff_morphism. intros Hfm1eqfm2.
 
 
       rewrite equal_iff_interpr_same. 2: apply M_satisfies_theory.
@@ -804,13 +843,7 @@ Section sorts.
       rewrite update_evar_val_neq.
       { solve_fresh_neq. }
       rewrite update_evar_val_same.
-      repeat rewrite pattern_interpretation_free_evar_independent.
-      1-2: rewrite Heqx₁; clear; eapply evar_is_fresh_in_richer; [|apply set_evar_fresh_is_fresh]; set_solver.
-      apply all_iff_morphism. intros Hfm1eqfm2.
       clear. set_solver.
-      { eapply well_formed_closed_ex_aux_ind. 2: eassumption. lia. }
-      { rewrite bevar_subst_not_occur; auto; simpl. eapply well_formed_closed_ex_aux_ind. 2: eassumption. lia. }
-      { auto. }
     Qed.
 
 
